new-backend/bvl_to_bvpScript.sml
@@ -52,10 +52,11 @@ val bComp_def = tDefine "bComp" `
      let (c1,v1,n1) = bComp n env F live [x1] in
        (Seq c1 (Raise (HD v1)), v1, n1)) /\
   (bComp n env tail live [Handle x1 x2] =
+     let ns = list_to_num_set (live ++ env) in
      let (c1,v1,n1) = bComp n env F live [x1] in
      let (c2,v2,n2) = bComp (n1+1) (n1::env) F live [x2] in
-     let c3 = Handle (Seq c1 (Move n2 (HD v1))) n2 n1
-                     (Seq c2 (Move n2 (HD v2))) in
+     let c3 = Handle ns (Seq c1 (Move n2 (HD v1))) n2 n1
+                     ns (Seq c2 (Move n2 (HD v2))) in
        (if tail then Seq c3 (Return n2) else c3, [n2], n2+1)) /\
   (bComp n env tail live [Op op xs] =
      let (c1,vs,n1) = bComp n env F live xs in
@@ -251,7 +252,7 @@ val jump_exc_IMP = prove(
   \\ fs [] \\ Cases_on `h'` \\ fs [] \\ Cases_on `h` \\ fs [])
 
 val jump_exc_push_exc = prove(
-  ``jump_exc (push_exc t1) <> NONE``,
+  ``jump_exc (push_exc env1 env2 t1) <> NONE``,
   fs [jump_exc_def,push_exc_def,Q.SPEC `y::x::xs` LAST_N_LENGTH
            |> SIMP_RULE std_ss [LENGTH,ADD1]] \\ fs [] \\ DECIDE_TAC);
 
@@ -342,6 +343,18 @@ val MEM_LIST_REL = prove(
   ``!xs ys P x. LIST_REL P xs ys /\ MEM x xs ==> ?y. MEM y ys /\ P x y``,
   Induct \\ Cases_on `ys` \\ fs [] \\ REPEAT STRIP_TAC \\ fs []
   \\ RES_TAC \\ METIS_TAC []);
+
+val lookup_inter_EQ = prove(
+  ``((lookup x (inter t1 t2) = SOME y) <=>
+       (lookup x t1 = SOME y) /\ lookup x t2 <> NONE) /\
+    ((lookup x (inter t1 t2) = NONE) <=>
+       (lookup x t1 = NONE) \/ (lookup x t2 = NONE))``,
+  fs [lookup_inter] \\ REPEAT BasicProvers.CASE_TAC);
+
+val LIST_REL_MEM = prove(
+  ``!xs ys P. LIST_REL P xs ys <=>
+              LIST_REL (\x y. MEM x xs /\ MEM y ys ==> P x y) xs ys``,
+  fs [LIST_REL_EL_EQN] \\ METIS_TAC [MEM_EL]);
 
 val bComp_correct = prove(
   ``!xs env s1 res s2 t1 n corr tail live.
@@ -630,13 +643,28 @@ val bComp_correct = prove(
     \\ FULL_SIMP_TAC std_ss [pEval_def]
     \\ Cases_on `bEval ([x1],env,s1)` \\ fs []
     \\ Cases_on `q` \\ fs [isException_def,isResult_def]
-    \\ FIRST_X_ASSUM (MP_TAC o Q.SPECL [`push_exc t1`,`n`,`corr`,`F`,`live`])
-    \\ `var_corr env corr (push_exc t1) /\
-        state_rel s1 (push_exc t1) /\
-        !k. n <= k ==> lookup k (push_exc t1).locals = NONE` by
-          fs [var_corr_def,push_exc_def,get_var_def,state_rel_def]
-    \\ `EVERY (\n. lookup n (push_exc t1).locals <> NONE) live` by
-         fs [EVERY_MEM,push_exc_def]
+    \\ `domain (list_to_num_set (live ++ corr)) SUBSET domain t1.locals` by
+     (fs [SUBSET_DEF,domain_lookup,lookup_list_to_num_set,EVERY_MEM]
+      \\ REPEAT STRIP_TAC \\ RES_TAC THEN1
+       (`lookup x t1.locals <> NONE` by METIS_TAC []
+        \\ Cases_on `lookup x t1.locals` \\ fs [] \\ METIS_TAC [])
+      \\ fs [var_corr_def,get_var_def]
+      \\ IMP_RES_TAC MEM_LIST_REL \\ fs [])
+    \\ fs [cut_env_def]
+    \\ Q.ABBREV_TAC `env1 = (inter t1.locals (list_to_num_set (live ++ corr)))`
+    \\ FIRST_X_ASSUM (MP_TAC o Q.SPECL [`push_exc env1 env1 t1`,
+         `n`,`corr`,`F`,`live`])
+    \\ `var_corr env corr (push_exc env1 env1 t1) /\
+        state_rel s1 (push_exc env1 env1 t1) /\
+        !k. n <= k ==> lookup k (push_exc env1 env1 t1).locals = NONE` by
+         (UNABBREV_ALL_TAC
+          \\ fs [var_corr_def,push_exc_def,get_var_def,state_rel_def,
+                 lookup_inter_EQ,lookup_list_to_num_set]
+          \\ Q.PAT_ASSUM `LIST_REL rrr xs1 xs2` MP_TAC
+          \\ ONCE_REWRITE_TAC [LIST_REL_MEM] \\ fs [] \\ NO_TAC)
+    \\ `EVERY (\n. lookup n (push_exc env1 env1 t1).locals <> NONE) live` by
+        (UNABBREV_ALL_TAC \\ fs [EVERY_MEM,push_exc_def,
+           lookup_inter_EQ,lookup_list_to_num_set] \\ NO_TAC)
     \\ fs [] \\ REPEAT STRIP_TAC \\ fs [LET_DEF,jump_exc_push_exc]
     \\ Cases_on `pres` \\ fs []
     \\ IMP_RES_TAC bEval_SING_IMP \\ FULL_SIMP_TAC (srw_ss()) []
@@ -659,14 +687,17 @@ val bComp_correct = prove(
              \\ `k < LENGTH corr /\ n1 <= n2` by DECIDE_TAC \\ RES_TAC
              \\ REPEAT STRIP_TAC \\ fs [])
       THEN1 (Cases_on `k = n2` \\ fs [] \\ res_tac \\ DECIDE_TAC)
-      THEN1 (res_tac \\ SRW_TAC [] []
+      THEN1 (`lookup k env1 = SOME x` by (UNABBREV_ALL_TAC
+               \\ fs [lookup_inter_EQ,lookup_list_to_num_set]
+               \\ CCONTR_TAC \\ fs [])
+             \\ res_tac \\ SRW_TAC [] []
              \\ res_tac \\ SRW_TAC [] [] \\ `F` by DECIDE_TAC)
       \\ POP_ASSUM MP_TAC
       \\ Cases_on `jump_exc t1` \\ fs []
       \\ IMP_RES_TAC jump_exc_IMP \\ fs [jump_exc_def])
     THEN1 (* not tail, body of handle raises exception *)
      (`(t2.stack = t1.stack) /\
-       (t2.handler = t1.handler) /\ (t2.locals = t1.locals)` by
+       (t2.handler = t1.handler) /\ (t2.locals = env1)` by
        (IMP_RES_TAC jump_exc_IMP \\ POP_ASSUM (fn th => ONCE_REWRITE_TAC [th])
         \\ POP_ASSUM MP_TAC \\ fs [push_exc_def]
         \\ fs [jump_exc_def,push_exc_def,Q.SPEC `y::x::xs` LAST_N_LENGTH
@@ -680,15 +711,17 @@ val bComp_correct = prove(
           \\ FULL_SIMP_TAC std_ss [listTheory.LIST_REL_EL_EQN]
           \\ REPEAT STRIP_TAC
           \\ Q.MATCH_ASSUM_RENAME_TAC `k < LENGTH env` []
-          \\ `EL k corr <> n1` by ALL_TAC \\ fs [lookup_insert]
+          \\ `EL k corr <> n1` by ALL_TAC \\ UNABBREV_ALL_TAC
+          \\ fs [lookup_insert,lookup_inter_EQ,lookup_list_to_num_set]
           \\ `k < LENGTH corr /\ n <= n1` by DECIDE_TAC \\ RES_TAC
-          \\ REPEAT STRIP_TAC \\ fs [])
+          \\ REPEAT STRIP_TAC \\ fs [] \\ METIS_TAC [MEM_EL])
         THEN1 (fs [set_var_def,lookup_insert]
           \\ SRW_TAC [] [] THEN1 DECIDE_TAC
-          \\ `n <= k` by DECIDE_TAC \\ RES_TAC)
+          \\ `n <= k` by DECIDE_TAC
+          \\ UNABBREV_ALL_TAC \\ fs [lookup_inter_EQ] \\ RES_TAC)
         \\ fs [state_rel_def,set_var_def,jump_exc_NONE,lookup_insert]
         \\ IMP_RES_TAC jump_exc_IMP_jump_exc
-        \\ fs [EVERY_MEM] \\ SRW_TAC [] [])
+        \\ fs [EVERY_MEM,push_exc_def] \\ SRW_TAC [] [])
       \\ STRIP_TAC \\ fs []
       \\ REVERSE (Cases_on `pres`) \\ fs [set_var_def] THEN1 (METIS_TAC [])
       \\ Cases_on `res` \\ fs []
@@ -709,12 +742,15 @@ val bComp_correct = prove(
              \\ REPEAT STRIP_TAC \\ fs [])
       THEN1 (Cases_on `k = n2` \\ fs [] \\ res_tac \\ DECIDE_TAC)
       THEN1 (Cases_on `n <= k` THEN1 (RES_TAC \\ fs [push_exc_def])
-             \\ `k <> n2 /\ k <> n1` by DECIDE_TAC \\ fs [])
+             \\ `k <> n2 /\ k <> n1` by DECIDE_TAC \\ fs []
+             \\ FIRST_X_ASSUM MATCH_MP_TAC \\ UNABBREV_ALL_TAC
+             \\ fs [lookup_inter_EQ,lookup_list_to_num_set]
+             \\ CCONTR_TAC \\ fs [])
       \\ fs [var_corr_def,get_var_def]
       \\ POP_ASSUM MP_TAC
       \\ Cases_on `jump_exc t1` \\ fs []
       \\ IMP_RES_TAC jump_exc_IMP \\ fs [jump_exc_def])
-    THEN1
+    THEN1 (* tail, body of handle returns normally *)
      (POP_ASSUM (K ALL_TAC)
       \\ `get_var v1 t2 = SOME w` by fs [get_var_def,var_corr_def]
       \\ fs [get_var_def,set_var_def]
@@ -722,9 +758,9 @@ val bComp_correct = prove(
       \\ Q.PAT_ASSUM `x11 = t2.handler` (ASSUME_TAC o GSYM)
       \\ fs [pop_exc_def,push_exc_def,state_rel_def,var_corr_def,
              get_var_def,call_env_def,lookup_insert,res_list_def])
-    THEN1
+    THEN1 (* tail, body of handle raises exception *)
      (`(t2.stack = t1.stack) /\
-       (t2.handler = t1.handler) /\ (t2.locals = t1.locals)` by
+       (t2.handler = t1.handler) /\ (t2.locals = env1)` by
        (IMP_RES_TAC jump_exc_IMP \\ POP_ASSUM (fn th => ONCE_REWRITE_TAC [th])
         \\ POP_ASSUM MP_TAC \\ fs [push_exc_def]
         \\ fs [jump_exc_def,push_exc_def,Q.SPEC `y::x::xs` LAST_N_LENGTH
@@ -738,15 +774,17 @@ val bComp_correct = prove(
           \\ FULL_SIMP_TAC std_ss [listTheory.LIST_REL_EL_EQN]
           \\ REPEAT STRIP_TAC
           \\ Q.MATCH_ASSUM_RENAME_TAC `k < LENGTH env` []
-          \\ `EL k corr <> n1` by ALL_TAC \\ fs [lookup_insert]
+          \\ `EL k corr <> n1` by ALL_TAC \\ UNABBREV_ALL_TAC
+          \\ fs [lookup_insert,lookup_inter_EQ,lookup_list_to_num_set]
           \\ `k < LENGTH corr /\ n <= n1` by DECIDE_TAC \\ RES_TAC
-          \\ REPEAT STRIP_TAC \\ fs [])
+          \\ REPEAT STRIP_TAC \\ fs [] \\ METIS_TAC [MEM_EL])
         THEN1 (fs [set_var_def,lookup_insert]
           \\ SRW_TAC [] [] THEN1 DECIDE_TAC
-          \\ `n <= k` by DECIDE_TAC \\ RES_TAC)
+          \\ `n <= k` by DECIDE_TAC
+          \\ UNABBREV_ALL_TAC \\ fs [lookup_inter_EQ] \\ RES_TAC)
         \\ fs [state_rel_def,set_var_def,jump_exc_NONE,lookup_insert]
         \\ IMP_RES_TAC jump_exc_IMP_jump_exc
-        \\ fs [EVERY_MEM] \\ SRW_TAC [] [])
+        \\ fs [EVERY_MEM,push_exc_def] \\ SRW_TAC [] [])
       \\ STRIP_TAC \\ fs []
       \\ REVERSE (Cases_on `pres`) \\ fs [set_var_def] THEN1 (METIS_TAC [])
       \\ Cases_on `res` \\ fs []
